refactor + simple add

src/Dafny/control_flow.i.dfy
@@ -1,6 +1,6 @@
 include "llvm.i.dfy"
 
-module test {
+module control_flow {
     import opened LLVM_def
 
 predicate{:opaque} evalCodeOpaque(c:code, s0:state, sN:state,o:operand) 
@@ -206,121 +206,5 @@ predicate lvm_state_eq(s0:lvm_state, s1:lvm_state)
  && s0.gvs == s1.gvs
  && s0.m == s1.m
 }
-
-function method{:opaque} lvm_code_Empty_Test():lvm_code
-{   
-    lvm_Block(lvm_CNil())
-}       
-
-lemma lvm_lemma_Empty_Test(lvm_b0:lvm_codes, lvm_s0:lvm_state, lvm_sN:lvm_state, src:lvm_operand_opr,o:operand)
-  returns (lvm_bM:lvm_codes, lvm_sM:lvm_state)
-  requires lvm_require(lvm_b0, lvm_code_Empty_Test(), lvm_s0, lvm_sN,o)
-  requires lvm_is_src_opr(src, lvm_s0)
-  requires lvm_get_ok(lvm_s0)
-  ensures  lvm_ensure(lvm_b0, lvm_bM, lvm_s0, lvm_sM, lvm_sN,o)
-  ensures  lvm_get_ok(lvm_sM)
-  ensures  lvm_state_eq(lvm_sM, lvm_s0)
-ensures lvm_state_eq(lvm_sM, lvm_update_mem( lvm_sM, lvm_update_ok(lvm_sM, lvm_sM)))
-{
-  reveal_lvm_code_Empty_Test();
-  reveal_eval_code();
-  var lvm_old_s:lvm_state := lvm_s0;
-
-  assert lvm_s0.ok;
-  assert lvm_code_Empty_Test() == Block(CNil);
-  assert lvm_b0.hd == lvm_code_Empty_Test();
-  assert !lvm_b0.CNil?;
-  assert lvm_code_Empty_Test().block.CNil?;
-  assert lvm_b0.hd.Block?;
-  assert lvm_get_block(lvm_b0.hd).CNil?;
-  assert evalBlock(lvm_get_block(lvm_b0.hd),lvm_s0, lvm_s0,o);
-  assert forall r :: r == lvm_s0 ==> eval_code(lvm_b0.hd,lvm_s0,r,o);
-  assert evalCode_lax(Block(lvm_b0), lvm_s0, lvm_sN, o);
-//   assert exists r' :: evalBlock(lvm_b0.tl, lvm_s0, r',o);
-// assert Block(CNil).CNil?;
-assert evalBlock(lvm_b0, lvm_s0, lvm_sN,o) ==> exists r' :: evalCode(lvm_b0.hd, lvm_s0, r',o) && evalBlock(lvm_b0.tl, r', lvm_sN,o);
-assert exists r' :: if evalCode(lvm_b0.hd, lvm_s0, r',o) then true else true;
-// assert eval_code(Block(lvm_b0), lvm_s0, lvm_s0,o);
-//   assert evalBlock(lvm_b0, lvm_s0, lvm_sN,o);
-  
-//   assert eval_code(Block(lvm_b0), lvm_s0, lvm_sN,o);
-  ghost var lvm_ltmp1, lvm_cM:lvm_code, lvm_ltmp2 := lvm_lemma_block_lax(lvm_b0, lvm_s0, lvm_sN,o);
-  lvm_sM := lvm_ltmp1;
-  lvm_bM := lvm_ltmp2;
-  var lvm_b1:lvm_codes := lvm_get_block(lvm_cM);
-  assert evalCode_lax(lvm_Block(lvm_CNil()), lvm_s0, lvm_sM, o);
-
-  lvm_sM := lvm_lemma_empty(lvm_s0, lvm_sM);
-}
-
-function method{:opaque} lvm_code_Add(dst:lvm_operand_opr, size:nat, src1:lvm_operand_opr):lvm_code
-{
-    reveal_IntFits();
-    var val := D(Int(4,IntType(1,false)));
-    assert val.d.Int?;
-    // assert lvm_Block(lvm_CCons(Ins(ADD(dst, size,src1,val)),lvm_CNil())).Ins?;
-    lvm_Block(lvm_CCons(Ins(ADD(dst, size,src1,val)),lvm_CNil()))
-
-}
-
-lemma lvm_lemma_Add(lvm_b0:lvm_codes, lvm_s0:lvm_state, lvm_sN:lvm_state, 
-            dst:lvm_operand_opr, size:nat, src1:lvm_operand_opr,src2:lvm_operand_opr,o:operand)
-  returns (lvm_bM:lvm_codes, lvm_sM:lvm_state)
-  requires lvm_require(lvm_b0, lvm_code_Add(dst, size,src1), lvm_s0, lvm_sN,dst)
-  requires lvm_is_dst_opr(dst, lvm_s0)
-  requires lvm_is_src_opr(src1, lvm_s0)
-  requires lvm_get_ok(lvm_s0)
-
-  requires ValidOperand(lvm_s0,src1);
-  requires OperandContents(lvm_s0,src1).Int?;
-  requires lvm_code_Add(dst, size,src1).Ins?;
-//   requires ValidInstruction(lvm_s0,lvm_code_Add(dst, size,src1).ins);
-//   requires o == dst;
-  requires dst.LV?;
-//   
-  ensures  lvm_ensure(lvm_b0, lvm_bM, lvm_s0, lvm_sM, lvm_sN,dst)
-  ensures  lvm_get_ok(lvm_sM)
-  ensures OperandContents(lvm_sM,dst).Int?;
-  ensures OperandContents(lvm_s0,dst).Int?;
-
-  ensures  OperandContents(lvm_sM, dst).val == OperandContents(lvm_s0, dst).val + 4
-  ensures  lvm_state_eq(lvm_sM, lvm_update_ok(lvm_sM, lvm_update_mem( lvm_sM, lvm_s0)))
-{
-  reveal_lvm_code_Add();
-  assert lvm_code_Add(dst, size,src1).Ins?;
-  var addIns := lvm_code_Add(dst, size,src1).ins;
-  assert ValidInstruction(lvm_s0,addIns);
-//   assert o == dst;
-  assert  ValidRegOperand(lvm_s0, dst);
-  assert ValidState(lvm_s0);
-
-//   assert  OperandContents(lvm_s0,src1).Int?;
-//   assert evalADD(size,OperandContents(lvm_s0,src1),OperandContents(lvm_s0,src2)).Int?;
-// reveal_IntFits();
-//     var val := Int(4,IntType(1,false));
-//     assert val.Int?;
-    //   assert dst.LV?;
-    //   assert (lvm_sN == lvm_s0.(lvs := lvm_s0.lvs[o.l := evalADD(size,OperandContents(lvm_s0,src1),val)])) ==> evalUpdate(lvm_s0, dst, evalADD(size,OperandContents(lvm_s0,src1),val), lvm_sN); 
-//   assert lvm_s0 == lvm_sN;
-//   assert  evalIns(addIns, lvm_s0, lvm_sN,o);
- assert lvm_b0.hd.Ins?;
- 
-  var lvm_old_s:lvm_state := lvm_s0;
-//   lvm_ins_lemma(Ins(InsAdd(dst, src)), lvm_s0);
-  ghost var lvm_ltmp1, lvm_cM:lvm_code, lvm_ltmp2 := lvm_lemma_block_lax(lvm_b0, lvm_s0, lvm_sN,dst);
-  lvm_sM := lvm_ltmp1;
-  lvm_bM := lvm_ltmp2;
-  assert lvm_b0.tl == lvm_bM;
-  assert lvm_bM.CNil?;
-  assert  OperandContents(lvm_sM, dst).Int?;
-
-  assert evalCode_lax(lvm_cM, lvm_s0, lvm_sM,dst);
-  assert OperandContents(lvm_sM, dst).val == OperandContents(lvm_s0, dst).val + 4;
-//   assert ValidInstruction(lvm_s0,lvm_code_Add(dst, size,src1,src2).ins) ==> lvm_sM.ok;
-//   assert evalUpdate(lvm_s0, o, evalADD(size,OperandContents(lvm_s0,src1),val), lvm_sM);
-
-  reveal_evalCodeOpaque();
-}
-
 
 }   
